even_odd: progress

theories/examples/even_odd.v
@@ -20,6 +20,7 @@ Definition is_odd_code (x : string) : C_lang.expr :=
 Definition is_odd_func : C_lang.function :=
   Fun [BNamed "x"] (is_odd_code "x").
 
+
 Section specs.
 Context `{!heapGS_gen hlc Σ}.
 
@@ -49,6 +50,54 @@ Proof.
   iIntros (?). iStartProof.
   rewrite /is_even_code /=. cbn; simplify_map_eq.
   Fail wp_pures.
-Abort.
+Admitted.
+
+Lemma is_odd_spec (x:Z) E :
+  (0 ≤ x)%Z →
+  ⊢ WP subst "x" (#x) (is_odd_code "x") @ odd_env; E
+      {{ λ v, ⌜v = #(Z.odd x)⌝ }}.
+Admitted.
 
 End specs.
+
+From melocoton.interop Require Import linking linking_wp embed_wp.
+From melocoton.mlanguage Require Import weakestpre.
+
+Section linking.
+Context `{!heapGS_gen hlc Σ}.
+Context `{!linkGS Σ}.
+
+Definition penv : prog_environ (link_lang C_mlang C_mlang) Σ := {|
+  penv_prog := {[ "is_even" := inl is_even_func; "is_odd" := inr is_odd_func ]};
+  penv_proto := (λ _ _ _, False)%I;
+|}.
+
+Instance penv_is_link : is_link_environ (penv_to_mlang even_env) (penv_to_mlang odd_env) penv.
+Proof.
+  constructor.
+  { set_solver. }
+  { simpl. rewrite !fmap_insert !fmap_empty // -insert_union_l.
+    rewrite left_id_L //. }
+  { iIntros (? ? ? ? ? ?) "(-> & HT)". simpl in H.
+    iDestruct "HT" as (x [-> ?]) "HΦ".
+    iExists _. iSplitR.
+    { iPureIntro. simpl.
+      rewrite (_: func = is_odd_func); [|by simplify_map_eq/=].
+      rewrite /is_odd_func /apply_function. reflexivity. }
+    iIntros "!> _". iApply wp_wand.
+    { iApply wp_embed. by iApply is_odd_spec. }
+    iIntros (? ->). iFrame. }
+  { iIntros (? ? ? ? ? ?) "(-> & HT)". simpl in H.
+    iDestruct "HT" as (x [-> ?]) "HΦ".
+    iExists _. iSplitR.
+    { iPureIntro. simpl.
+      rewrite (_: func = is_even_func); [| by simplify_map_eq/=].
+      rewrite /is_even_func /apply_function. reflexivity. }
+    iIntros "!> _". iApply wp_wand.
+    { iApply wp_embed. by iApply is_even_spec. }
+    iIntros (? ->). iFrame. }
+  { iIntros (? ? ? ? ?) "(-> & _)". simplify_map_eq/=. }
+  { iIntros (? ? ? ? ?) "(-> & _)". simplify_map_eq/=. }
+Qed.
+
+End linking.
